wip

proofmode/HPSim.v
@@ -194,7 +194,7 @@ Section SIM.
   		_hpsim hpsim true true (st_src, i_src) (st_tgt, i_tgt) fmr
 	.
 
-	Lemma _hpsim_ind2
+	(* Lemma _hpsim_ind2
 				(hpsim: bool -> bool -> Any.t * itree hAGEs Any.t -> Any.t * itree hAGEs Any.t -> Σ -> Prop)
 				(P: bool -> bool -> Any.t * itree hAGEs Any.t -> Any.t * itree hAGEs Any.t -> Σ -> Prop)
 				(RET: forall
@@ -347,14 +347,14 @@ Section SIM.
 		{ eapply GUARANTEESRC; esplits; et. }
 		{ eapply GUARANTEETGT; esplits; et. }
 		{ eapply PROGRESS; eauto. }
-		Qed.
+		Qed. *)
 
 		Definition hpsim := paco5 _hpsim bot5.
 
 
 		Lemma _hpsim_mon: monotone5 _hpsim.
 		Proof. 
-			ii. induction IN using _hpsim_ind2;
+			ii. induction IN;
 			try (econs; et; ii; exploit K; i; des; et).
 		Qed.
 	
@@ -362,7 +362,6 @@ Section SIM.
 		Hint Unfold hpsim.
 		Hint Resolve _hpsim_mon: paco.
 		Hint Resolve cpn5_wcompat: paco.
-
 
 		Lemma hpsim_ind
 				(P: bool -> bool -> Any.t * itree hAGEs Any.t -> Any.t * itree hAGEs Any.t -> Σ -> Prop)
@@ -498,7 +497,7 @@ Section SIM.
 				(SIM: hpsim f_src f_tgt st_src st_tgt fmr),
 				P f_src f_tgt st_src st_tgt fmr.
 	Proof. 
-    i. punfold SIM. induction SIM using _hpsim_ind2.
+    i. punfold SIM. induction SIM.
 			{ eapply RET; eauto. }
 			{ eapply CALL; eauto. i. hexploit K; et. i. des. esplits; et. }
 			{ eapply SYSCALL; eauto. i. hexploit K; et. i. des. esplits; et. }
@@ -519,34 +518,281 @@ Section SIM.
 			{ eapply PROGRESS; eauto. pclearbot. et. }
 	Qed.
 
+  (* Variant hpsim_indC
+	(hpsim: bool -> bool -> Any.t * itree hAGEs Any.t -> Any.t * itree hAGEs Any.t -> Σ -> Prop)
+		: bool -> bool -> Any.t * itree hAGEs Any.t -> Any.t * itree hAGEs Any.t -> Σ -> Prop :=
+		(hpsim: bool -> bool -> Any.t * itree hAGEs Any.t -> Any.t * itree hAGEs Any.t -> Σ -> Prop)
+		: bool -> bool -> Any.t * itree hAGEs Any.t -> Any.t * itree hAGEs Any.t -> Σ -> Prop :=
+	| hpsim_ret
+			f_src f_tgt st_src st_tgt fmr
+			v_src v_tgt
+			(RET: current_iProp fmr (I st_src st_tgt))
+		:
+			_hpsim hpsim f_src f_tgt (st_src, Ret v_src) (st_tgt, Ret v_tgt) fmr
+
+	| hpsim_call
+			f_src f_tgt st_src st_tgt fmr
+			fn varg k_src k_tgt FR
+      (INV: current_iProp fmr (I st_src st_tgt ** FR))
+			(K: forall vret st_src0 st_tgt0 fmr0
+          (INV: current_iProp fmr0 (I st_src0 st_tgt0 ** FR)),
+				_hpsim hpsim true true (st_src0, k_src vret) (st_tgt0, k_tgt vret) fmr0)				
+		:
+			_hpsim hpsim f_src f_tgt (st_src, trigger (Call fn varg) >>= k_src) (st_tgt, trigger (Call fn varg) >>= k_tgt) fmr
+
+	| hpsim_syscall
+			f_src f_tgt st_src st_tgt fmr
+			fn varg rvs k_src k_tgt
+			(K: forall vret, 
+				_hpsim hpsim true true (st_src, k_src vret) (st_tgt, k_tgt vret) fmr)
+		:
+			_hpsim hpsim f_src f_tgt (st_src, trigger (Syscall fn varg rvs) >>= k_src) (st_tgt, trigger (Syscall fn varg rvs) >>= k_tgt) fmr
+
+	| hpsim_inline_src
+			f_src f_tgt st_src st_tgt fmr
+			fn f varg k_src i_tgt
+			(FUN: alist_find fn fl_src = Some f)
+			(K: _hpsim hpsim true f_tgt (st_src, (f varg) >>= k_src) (st_tgt, i_tgt) fmr)
+		:
+			_hpsim hpsim f_src f_tgt (st_src, trigger (Call fn varg) >>= k_src) (st_tgt, i_tgt) fmr
+
+	| hpsim_inline_tgt
+			f_src f_tgt st_src st_tgt fmr
+			fn f varg i_src k_tgt
+		  (FUN: alist_find fn fl_tgt = Some f)
+		  (K: _hpsim hpsim f_src true (st_src, i_src) (st_tgt, (f varg) >>= k_tgt) fmr)
+	  :
+		  _hpsim hpsim f_src f_tgt (st_src, i_src) (st_tgt, trigger (Call fn varg) >>= k_tgt) fmr
+
+	| hpsim_tau_src
+			f_src f_tgt st_src st_tgt fmr
+		  i_src i_tgt
+  		(K: _hpsim hpsim true f_tgt (st_src, i_src) (st_tgt, i_tgt) fmr)
+	  :
+		  _hpsim hpsim f_src f_tgt (st_src, tau;; i_src) (st_tgt, i_tgt) fmr
+
+	| hpsim_tau_tgt
+			f_src f_tgt st_src st_tgt fmr
+		  i_src i_tgt
+		  (K: _hpsim hpsim f_src true (st_src, i_src) (st_tgt, i_tgt) fmr)
+	  :
+		  _hpsim hpsim f_src f_tgt (st_src, i_src) (st_tgt, tau;; i_tgt) fmr
+
+	| hpsim_choose_src
+			f_src f_tgt st_src st_tgt fmr
+		  X x k_src i_tgt
+		  (K: _hpsim hpsim true f_tgt (st_src, k_src x) (st_tgt, i_tgt) fmr)
+  	:
+	  	_hpsim hpsim f_src f_tgt (st_src, trigger (Choose X) >>= k_src) (st_tgt, i_tgt) fmr
+
+	| hpsim_choose_tgt
+			f_src f_tgt st_src st_tgt fmr
+		  X i_src k_tgt
+		  (K: forall (x: X), _hpsim hpsim f_src true (st_src, i_src) (st_tgt, k_tgt x) fmr)
+	  :
+		  _hpsim hpsim f_src f_tgt (st_src, i_src) (st_tgt, trigger (Choose X) >>= k_tgt) fmr
+
+	| hpsim_take_src
+			f_src f_tgt st_src st_tgt fmr
+		  X k_src i_tgt
+		  (K: forall (x: X), _hpsim hpsim true f_tgt (st_src, k_src x) (st_tgt, i_tgt) fmr)
+	  :
+		  _hpsim hpsim f_src f_tgt (st_src, trigger (Take X) >>= k_src) (st_tgt, i_tgt) fmr
+
+	| hpsim_take_tgt
+			f_src f_tgt st_src st_tgt fmr
+		  X x i_src k_tgt
+		  (K: _hpsim hpsim f_src true (st_src, i_src) (st_tgt, k_tgt x) fmr)
+	  :
+		  _hpsim hpsim f_src f_tgt (st_src, i_src) (st_tgt, trigger (Take X) >>= k_tgt) fmr
+
+	| hpsim_supdate_src
+			f_src f_tgt st_src st_tgt fmr
+      X x st_src0 k_src i_tgt
+      (run: Any.t -> Any.t * X)
+      (RUN: run st_src = (st_src0, x))
+		  (K: _hpsim hpsim true f_tgt (st_src0, k_src x) (st_tgt, i_tgt) fmr)
+	  :
+		  _hpsim hpsim f_src f_tgt (st_src, trigger (SUpdate run) >>= k_src) (st_tgt, i_tgt) fmr
+
+	| hpsim_supdate_tgt
+			f_src f_tgt st_src st_tgt fmr
+      X x st_tgt0 i_src k_tgt
+      (run: Any.t -> Any.t * X)
+      (RUN: run st_tgt = (st_tgt0, x))
+		  (K: _hpsim hpsim f_src true (st_src, i_src) (st_tgt0, k_tgt x) fmr)
+	  :
+		  _hpsim hpsim f_src f_tgt (st_src, i_src) (st_tgt, trigger (SUpdate run) >>= k_tgt) fmr
+
+	| hpsim_assume_src
+			f_src f_tgt st_src st_tgt fmr
+			iP k_src i_tgt FMR
+      (CUR: current_iProp fmr FMR)
+			(K: forall fmr0 (NEW: current_iProp fmr0 (iP ** FMR)),
+          _hpsim hpsim true f_tgt (st_src, k_src tt) (st_tgt, i_tgt) fmr0)
+		:
+			_hpsim hpsim f_src f_tgt (st_src, trigger (Assume iP) >>= k_src) (st_tgt, i_tgt) fmr
+
+	| hpsim_assume_tgt
+			f_src f_tgt st_src st_tgt fmr
+			iP i_src k_tgt FMR
+      (CUR: current_iProp fmr (iP ** FMR))
+			(K: forall fmr0 (NEW: current_iProp fmr0 FMR),
+          _hpsim hpsim f_src true (st_src, i_src) (st_tgt, k_tgt tt) fmr0)
+		:
+			_hpsim hpsim f_src f_tgt (st_src, i_src) (st_tgt, trigger (Assume iP) >>= k_tgt) fmr
+
+	| hpsim_guarantee_src
+			f_src f_tgt st_src st_tgt fmr
+			iP k_src i_tgt FMR
+      (CUR: current_iProp fmr (iP ** FMR))
+			(K: forall fmr0 (NEW: current_iProp fmr0 FMR),
+          _hpsim hpsim true f_tgt (st_src, k_src tt) (st_tgt, i_tgt) fmr0)
+		:
+			_hpsim hpsim f_src f_tgt (st_src, trigger (Guarantee iP) >>= k_src) (st_tgt, i_tgt) fmr
+
+	| hpsim_guarantee_tgt
+			f_src f_tgt st_src st_tgt fmr
+			iP i_src k_tgt FMR
+      (CUR: current_iProp fmr FMR)
+			(K: forall fmr0 (NEW: current_iProp fmr0 (iP ** FMR)),
+          _hpsim hpsim f_src true (st_src, i_src) (st_tgt, k_tgt tt) fmr0)
+		:
+			_hpsim hpsim f_src f_tgt (st_src, i_src) (st_tgt, trigger (Guarantee iP) >>= k_tgt) fmr
+
+	| hpsim_progress
+  		st_src st_tgt fmr
+      i_src i_tgt
+  		(SIM: hpsim false false (st_src, i_src) (st_tgt, i_tgt) fmr)
+  	:
+  		_hpsim hpsim true true (st_src, i_src) (st_tgt, i_tgt) fmr
+	.   *)
+
+	Lemma hpsim_bot_flag_up f_src f_tgt st_src st_tgt fmr
+			(SIM: paco5 _hpsim bot5 true true st_src st_tgt fmr)
+		:
+			paco5 _hpsim bot5 f_src f_tgt st_src st_tgt fmr
+	.
+	Proof.
+		ginit. 
+		do 2 remember true in SIM at 1.
+		clear Heqb Heqb0. 
+		revert_until I.
+		gcofix CIH.
+		i. revert f_src f_tgt.
+		pattern b, b0, st_src, st_tgt, fmr.
+		match goal with
+		| |- ?P b b0 st_src st_tgt fmr => set P
+		end.
+		revert b b0 st_src st_tgt fmr SIM.
+		eapply (@hpsim_ind P); subst P; ss; i; clarify.
+		{ gstep. econs; et. }
+		{ gstep. econs; et. i. hexploit K; et. i. des. econs. gfinal. left. eapply CIH. et. }
+		{ gstep. econs; et. i. hexploit K; et. i. des. econs. gfinal. left. eapply CIH. et. }
+	Admitted.	
+
+	Lemma current_iProp_sepconj P Q r 
+			(SAT: current_iProp r (P ** Q))
+		:
+			exists rp rq, URA.updatable r (rp ⋅ rq) /\ current_iProp rp P /\ current_iProp rq Q
+	.
+	Proof.
+		destruct SAT. rr in IPROP. uipropall. des. clarify.
+		hexploit UPD. i. eapply URA.updatable_wf in H; et. des.
+		esplits; et; econs; et; r_solve.
+		- eapply URA.wf_mon in H. et.
+		- eapply URA.wf_extends in H; et. econs. instantiate (1:= a). r_solve.
+	Qed.
+
+	Lemma current_iProp_sepconj' P Q r 
+			(SAT: current_iProp r (P ** Q))
+		:
+			exists rp rq, URA.updatable r (rp ⋅ rq) /\ P rp /\ Q rq
+	.
+	Proof.
+		destruct SAT. rr in IPROP. uipropall. des. clarify.
+		hexploit UPD. i. eapply URA.updatable_wf in H; et. 
+	Qed.
+
+	Lemma current_iProp_conj P Q x y
+			(IP: current_iProp x P)
+			(IQ: current_iProp y Q)
+			(WF: URA.wf (x ⋅ y))
+	:
+			current_iProp (x ⋅ y) (P ** Q)
+	.
+	Proof. 
+		inv IP. inv IQ.
+		econs; et.
+		{ uipropall. esplits; et. }
+		eapply URA.updatable_add; et.
+	Qed.
+
+
+  Lemma current_iPropL_convert fmr P
+        (CUR: current_iProp fmr P)
+    :
+      current_iPropL fmr [("H", P)].
+  Proof.
+    unfold current_iPropL. ss. unfold from_iPropL.
+    eapply current_iProp_entail; eauto.
+  Qed.
+
+
+	(* Move to HoareDef. *)
+	Lemma interp_hp_Assume
+      iP
+      fr
+  :
+    (interp_hp_tgt (trigger (Assume iP)) fr)
+    =
+		(* interp_state (handle_hAGE_tgt) (trigger (Assume iP)) fr *)
+    ('(fr, _) <- (handle_Assume iP fr);; tau;; Ret (fr, tt))
+.
+Proof.
+	unfold interp_hp_tgt, trigger. rewrite ! interp_state_vis. grind. rewrite u. et.
+Qed.
+
+	Lemma interp_hp_Guarantee
+      iP
+      fr
+  :
+    (interp_hp_tgt (trigger (Guarantee iP)) fr)
+    =
+		(* interp_state (handle_hAGE_tgt) (trigger (Assume iP)) fr *)
+    ('(fr', _) <- (handle_Guarantee iP fr);; tau;; Ret (fr', tt))
+.
+Proof.
+	unfold interp_hp_tgt, trigger. rewrite ! interp_state_vis. grind. rewrite u. et.
+Qed.
+
   Variant mk_inv  
           (I: Any.t -> Any.t -> iProp)
     : unit -> Any.t * Any.t -> Prop :=
   | mk_inv_intro
-      mr_src st_src mr_tgt st_tgt
+      (mr_src mr_tgt: Σ) st_src st_tgt
+			(* (MR: URA.extends mr_src mr_tgt) *)
+			(* (INV: exists mr, current_iProp mr (I st_src st_tgt)) *)
       (INV: 
-						(* forall (WF: URA.wf mr_src),  *)
-						exists MR_tgt,
-						<<MRS: current_iProp mr_src (I st_src st_tgt ** MR_tgt)>> /\
-						<<MRT: current_iProp mr_tgt MR_tgt>>)
+						exists mr,
+						(* <<MRS: mr_src = mr ⋅ mr_tgt>> /\		 *)
+						<<MR: current_iProp mr (I st_src st_tgt)>>)
     :
       mk_inv I tt (Any.pair st_src mr_src↑, Any.pair st_tgt mr_tgt↑)
   .
 
-	(* Check _sim_itree. *)
-
 
   Lemma hpsim_adequacy:
     forall
-      f_src f_tgt st_src st_tgt fl_src fl_tgt itr_src itr_tgt
-			(mr_src mr_tgt fr_src fr_tgt: Σ) FR FR_tgt
-      (SIM: hpsim f_src f_tgt (st_src, itr_src) (st_tgt, itr_tgt) (fr_src ⋅ mr_src))
-			(FRS: current_iProp fr_src (FR ** FR_tgt))
-			(FRT: current_iProp fr_tgt FR_tgt),
+      f_src f_tgt st_src st_tgt (fl_src0 fl_tgt0: alist string (Any.t -> itree Es Any.t)) itr_src itr_tgt
+			(mr_src mr_tgt fr_src fr_tgt fmr: Σ)
+      (SIM: hpsim f_src f_tgt (st_src, itr_src) (st_tgt, itr_tgt) fmr)
+			(FMR: fr_src ⋅ mr_src = fmr ⋅ fr_tgt ⋅ mr_tgt),
 
-			@sim_itree unit (mk_inv I) (fun _ _ => True) fl_src fl_tgt f_src f_tgt tt 
-			(Any.pair st_src mr_src↑, (interp_hp_tgt itr_src fr_src) >>= (fun r => Ret (snd r)))
-			(Any.pair st_tgt mr_tgt↑, (interp_hp_tgt itr_tgt fr_tgt) >>= (fun r => Ret (snd r))).
+
+			@sim_itree unit (mk_inv I) (fun _ _ => True) fl_src0 fl_tgt0 f_src f_tgt tt 
+			(Any.pair st_src mr_src↑, (interp_hp_tgt_fun itr_src fr_src) >>= (fun r => Ret (snd r)))
+			(Any.pair st_tgt mr_tgt↑, (interp_hp_tgt_fun itr_tgt fr_tgt) >>= (fun r => Ret (snd r))).
   Proof.
 		i. 
 		remember (Any.pair st_src mr_src↑). remember (Any.pair st_tgt mr_tgt↑).
@@ -554,10 +800,134 @@ Section SIM.
 		ginit. gcofix CIH. i.
 		remember (st_src, itr_src). remember (st_tgt, itr_tgt).
 		
-		revert st_src st_tgt itr_src itr_tgt Heqp Heqp0 Heqt Heqt0 CIH.
-		induction SIM using hpsim_ind; i; clarify.
-		- steps. econs; esplits; et. admit. admit.
-		- steps. { admit. } hexploit K; et. i. des. eapply IH.
+		(* revert st_src st_tgt itr_src itr_tgt Heqp Heqp0 Heqt Heqt0 CIH. *)
+		revert mr_src mr_tgt fr_src fr_tgt FMR st_src st_tgt itr_src itr_tgt Heqp Heqp0 Heqt Heqt0 CIH.
+
+		induction SIM using hpsim_ind; i; clarify; unfold interp_hp_tgt_fun, handle_Guarantee, mget, mput.
+		- steps.
+			force_l. instantiate (1 := (c0 ⋅ c1, ε, fmr ⋅ c)). steps.
+			unfold guarantee. force_l.
+			{ 
+				rewrite FMR. eapply URA.updatable_add in _GUARANTEE; r_solve.
+				etrans; [|etrans]; [|eassumption|]; try instantiate (1:= fmr);
+				erewrite (@f_equal2 _ _ _ URA.updatable); try refl; r_solve.
+			} 
+			steps. force_l. 
+			{ rr. uipropall. } 
+			steps. econs; esplits; et.
+			+ econs. esplits; et.
+			+ admit.
+		- hexploit INV. i. eapply current_iProp_sepconj' in H. des.
+			rename rq into fr. rename rp into mr.
+			steps.
+			{ econs. exists mr. esplits; et. econs; et. inv INV. eapply URA.updatable_wf in H; et. des. eapply URA.wf_mon.  et. r_solve. (* need mr_src = mr ⋅ mr_tgt *) }
+			inv WF. des.
+			unfold handle_Guarantee, mget, mput. steps.
+			force_l. 
+			instantiate (1:= (c0, fr ⋅ c1, mr0 ⋅ c)). 
+			steps.
+			unfold guarantee. force_l.
+			{ (* need fr_src ~> fr ⋅ fr_tgt *) admit. }  
+			steps. force_l.
+			{ rr. uipropall. }
+			steps. 
+			unfold interp_hp_tgt_fun, handle_Guarantee, mget, mput, guarantee in K.
+			remember (fr ⋅ c1). remember (mr0 ⋅ c). 
+			hexploit K.
+			{ 
+				eapply current_iProp_conj; [eapply MR|et|]. eapply URA.updatable_wf; et.
+				inv INV; et. etrans; et. admit. (* need mr -> mr0 updatable *)
+			}
+			i. des.
+			gstep. econs. gfinal. left. 
+			unfold interp_hp_tgt_fun, handle_Guarantee, mget, mput in *. rewrite <- ! bind_bind in *.
+			eapply CIH; et.
+			{ eapply hpsim_bot_flag_up. et. }
+			clarify. r_solve.
+		- steps. hexploit K; et. i. des.
+			unfold interp_hp_tgt_fun, handle_Guarantee, mget, mput in *. rewrite <- ! bind_bind in *.
+			eapply IH; et.
+		- steps. { admit. (* need to clarify the relation of fl_src ~ fl_src0 *) }
+			admit.
+		- admit. 
+		- steps. unfold interp_hp_tgt_fun, handle_Guarantee, mget, mput in *. rewrite <- ! bind_bind in *. et.
+		- steps. unfold interp_hp_tgt_fun, handle_Guarantee, mget, mput in *. rewrite <- ! bind_bind in *. et.
+		- steps. force_l. steps. unfold interp_hp_tgt_fun, handle_Guarantee, mget, mput in *. rewrite <- ! bind_bind in *. et.
+		- steps. hexploit K; et. i. des.
+			unfold interp_hp_tgt_fun, handle_Guarantee, mget, mput in *. rewrite <- ! bind_bind in *.
+			eapply IH; et.
+		- steps. hexploit K; et. i. des.
+			unfold interp_hp_tgt_fun, handle_Guarantee, mget, mput in *. rewrite <- ! bind_bind in *.
+			eapply IH; et.
+		- steps. force_r. steps. unfold interp_hp_tgt_fun, handle_Guarantee, mget, mput in *. rewrite <- ! bind_bind in *. et.
+		- steps. rewrite ! Any.pair_split. rewrite RUN. s.
+			(* unfold interp_hp_tgt_fun, handle_Guarantee, mget, mput in *. rewrite <- ! bind_bind in *. *)
+	
+			(* Ret r0.2 <- 'r0' (r0.1) changes.  *)
+			 admit.
+		- steps. rewrite ! Any.pair_split. rewrite RUN. s. admit.
+		- steps. rewrite interp_hp_Assume. unfold handle_Assume, mget, mput. steps.  
+			unfold interp_hp_tgt_fun, handle_Guarantee, mget, mput in *. rewrite <- ! bind_bind in *.
+			hexploit K; et.
+			{
+				eapply current_iProp_conj; et.
+				{ 
+					instantiate (1:= x). econs; [et| |r_solve].
+					do 2 eapply URA.wf_mon in _ASSUME. et.
+				}
+				assert (URA.wf (x ⋅ fmr ⋅ fr_tgt ⋅ mr_tgt)). 
+				{ 
+					replace (x ⋅ fmr ⋅ fr_tgt ⋅ mr_tgt) with (x ⋅ fr_src ⋅ mr_src); [eapply _ASSUME|r_solve]. 
+					rewrite URA.add_assoc. et.
+				}
+				do 2 eapply URA.wf_mon in H. et.
+			}
+			i. des. eapply IH; et.
+			rewrite <- ! URA.add_assoc.
+			f_equal.
+			rewrite URA.add_assoc. et.
+		-	steps. rewrite interp_hp_Assume. unfold handle_Assume, mget, mput. steps.
+			apply current_iProp_sepconj in CUR. des.
+
+			force_r. steps. unfold assume. force_r.
+			{ instantiate (1:= rp).  admit. }
+			steps. force_r.
+			{ admit. }
+			steps.
+			unfold interp_hp_tgt_fun, handle_Guarantee, mget, mput in *. rewrite <- ! bind_bind in *.
+			hexploit K; et. i. des. 
+			(* rewrite <- ! bind_bind in *. *)
+			(* unfold interp_hp_tgt_fun, handle_Guarantee, mget, mput in *.  *)
+
+			eapply IH; et. (* rp ⋅ rq ~ fmr : eq or updatable? *)		
+			admit.
+		- steps. rewrite interp_hp_Guarantee.
+			unfold handle_Guarantee, mget, mput. steps.
+			apply current_iProp_sepconj in CUR. des.
+			force_l. 
+			instantiate (1:= (rp, fr_src, mr_src)).  
+			steps. unfold guarantee at 1.
+			force_l.
+			{ admit. }
+			steps. unfold guarantee at 1. force_l.
+			{ admit.  }
+			steps.
+			hexploit K; et. i. des.
+			unfold interp_hp_tgt_fun, handle_Guarantee, mget, mput in *. rewrite <- ! bind_bind in *.
+			eapply IH; et.
+			admit.
+		- steps. rewrite interp_hp_Guarantee. unfold handle_Guarantee, mget, mput. 
+			steps. 
+			unfold interp_hp_tgt_fun, handle_Guarantee, mget, mput in *. rewrite <- ! bind_bind in *.
+			hexploit K; et.
+			{ instantiate (1:= (c0 ⋅ fmr)). admit. }
+			i. des.
+			replace c with mr_tgt.
+			eapply IH; et.
+
+			admit. admit.
+		- gstep. econs. gfinal. left. eapply CIH; et. 
+			(* (fr_src ⋅ mr_src) -> fmr in 'SIM' *)
 	Admitted.
 
 
