proofmode/HTactics.v
@@ -95,7 +95,7 @@ Section SIM.
       (SIM: exists w0,
           (<<WF: wf w0 (st_src0, st_tgt0)>>) /\
           (<<K: forall w1 vret st_src1 st_tgt1 (WLE: le w0 w1) (WF: wf w1 (st_src1, st_tgt1)),
-              g _ _ RR true true w (st_src1, k_src vret) (st_tgt1, k_tgt vret)>>))
+              r _ _ RR true true w (st_src1, k_src vret) (st_tgt1, k_tgt vret)>>))
     :
       _safe_sim_itree r g RR i_src0 i_tgt0 w (st_src0, trigger (Call fn varg) >>= k_src)
                       (st_tgt0, trigger (Call fn varg) >>= k_tgt)
@@ -104,7 +104,7 @@ Section SIM.
       i_src0 i_tgt0 w0 st_src0 st_tgt0
       fn varg rvs k_src k_tgt
       (K: forall vret,
-          g _ _ RR true true w0 (st_src0, k_src vret) (st_tgt0, k_tgt vret))
+          r _ _ RR true true w0 (st_src0, k_src vret) (st_tgt0, k_tgt vret))
     :
       _safe_sim_itree r g RR i_src0 i_tgt0 w0 (st_src0, trigger (Syscall fn varg rvs) >>= k_src)
                       (st_tgt0, trigger (Syscall fn varg rvs) >>= k_tgt)
